src/Result1.v
@@ -1,0 +1,37 @@
+From Pony Require Import Language Typing Heap Semantics.
+
+Require Import Coq.FSets.FMapInterface.
+Require Import Coq.MSets.MSetInterface.
+Require Import Coq.Structures.Equalities.
+
+Module Result1 (Map : WSfun) (SetM : WSetsOn).
+
+Module Sem := Semantics Map SetM.
+
+Theorem result1 :
+  forall P : Sem.WFExpr.Program.program,
+  forall gamma gamma' : Sem.WFExpr.context,
+  forall e : Syntax.expression,
+  forall E : Syntax.expressionSeq,
+  forall S : Syntax.typeId,
+  forall k : Syntax.capability,
+  forall T : Syntax.ponyType,
+  forall L L' : Sem.localVars,
+  forall chi chi' : Sem.heap,
+  forall v : Sem.value,
+    @Sem.WFExpr.typing P Syntax.expression gamma e (Syntax.type S k) gamma'
+    -> @Sem.WFExpr.well_formed_expr P gamma (Syntax.seq e E) T
+    -> (forall x : Syntax.var, 
+        forall S' : Syntax.typeId,
+        forall b : Syntax.baseCapability,
+        forall v' : Sem.value,
+          Sem.WFExpr.VarMapsTo x (Syntax.aType S' b) gamma
+          -> Sem.VarMap.MapsTo x v' L
+          -> Sem.heapTyping v' S' chi)
+    -> @Sem.evaluatesTo P Syntax.expression chi L e chi' L' v
+    -> Sem.heapTyping v S chi'
+        /\ @Sem.WFExpr.well_formed_expr P gamma' E T.
+Proof.
+  Admitted.
+
+End Result1.
